typeExtractionSem: simplify semantic equivalence and proofs
To simplify envD_equiv without breaking any lemma, what was crucial was changing
`interp_extractedTy` as well; this change would not have been possible without
switching logical relations to infinite substitutions.

theories/DSub/typeExtractionSem.v
@@ -30,12 +30,11 @@ Section interp_equiv.
   (** However, a stamp semantics that carries over to saved predicates must use
       σ in ρ. And the result is only equivalent for closed ρ with the expected length. *)
   Definition interp_extractedTy: (ty * vls) → envD Σ :=
-    λ '(T, σ) ρ v,
-    (⟦ T ⟧ (to_subst σ.|[ρ]) v)%I.
+    λ '(T, σ) ρ v, (⟦ T ⟧ (to_subst σ >> ρ) v)%I.
   Notation "⟦ T ⟧ [ σ ]" := (interp_extractedTy (T, σ)).
 
   Definition envD_equiv n φ1 φ2: iProp Σ :=
-    (∀ ρ v, ⌜ length ρ = n ⌝ → ⌜ cl_ρ ρ ⌝ → φ1 (to_subst ρ) v ≡ φ2 (to_subst ρ) v)%I.
+    (∀ ρ v, φ1 (to_subst ρ) v ≡ φ2 (to_subst ρ) v)%I.
   Notation "φ1 ≈[  n  ] φ2" := (envD_equiv n φ1 φ2) (at level 70).
 
   Lemma extraction_envD_equiv g s σ T n:
@@ -43,8 +42,9 @@ Section interp_equiv.
     (∃ T', ⌜ g !! s = Some T'⌝ ∧
         ⟦ T ⟧ ≈[ n ] ⟦ T' ⟧ [ σ ])%I.
   Proof.
-    iIntros ((T' & -> & <- & HclT & HclT')). iExists _; iSplit => //.
-    iIntros (ρ v <- Hclρ). by rewrite interp_subst_commute.
+    iIntros ((T' & -> & <- & _ & _)). iExists _; iSplit => //.
+    iIntros (ρ v) "!%".
+    rewrite /interp_extractedTy. exact: interp_subst_compose.
   Qed.
 
   (** envD_equiv commutes with substitution. *)
@@ -57,11 +57,12 @@ Section interp_equiv.
     ⟦ T1 ⟧ [ σ1.|[to_subst ξ] ] ≈[ n ] ⟦ T2 ⟧ [ σ2 ])%I.
   Proof.
     rewrite /interp_extractedTy; iIntros ((T1 & -> & Heq1 & Hclσ1 & HclT1) (T2 & -> & Heq2 & Hclσ2 & HclT2) Hlenξ Hclξ).
-    iExists _, _; repeat iSplit => //; iIntros (ρ v Hlenρ Hclρ) "/= !%"; subst.
-    have Hclσ1ξ: nclosed_σ σ1.|[to_subst ξ] (length ρ). exact: nclosed_σ_to_subst.
-    have Hrew: T2.|[to_subst σ2.|[to_subst ρ]] = T1.|[to_subst σ1.|[to_subst ξ].|[to_subst ρ]].
-    by erewrite !subst_compose; rewrite ?map_length ?Heq1 ?Heq2.
-    rewrite (interp_subst_ids T1 _ _) (interp_subst_ids T2 _ _) ?Hrew //; exact: nclosed_σ_to_subst.
+    iExists _, _; repeat iSplit => //; iIntros (ρ v) "/= !%".
+    have Hrew: T2.|[to_subst σ2].|[to_subst ρ] =
+      T1.|[to_subst σ1.|[to_subst ξ]].|[ to_subst ρ].
+    by erewrite !subst_compose, Heq2, Heq1.
+    asimpl in Hrew.
+    rewrite (interp_subst_ids T1 _ _) (interp_subst_ids T2 _ _) Hrew //.
   Qed.
 
   Lemma alloc_sp T: (|==> ∃ γ, γ ⤇ ty_interp T)%I.
